Crash safe log example (IV)

examples/log/DiskLogSystemCrashSafeLogRefinement.dfy
@@ -1,8 +1,9 @@
 include "CrashSafeLog.dfy"
-include "DiskLogSystem.dfy"
+include "DiskLogSystemInv.dfy"
 
 module DiskLogSystemCrashSafeLogRefinement {
-  import DLS = DiskLogSystemInv
+  import DLSI = DiskLogSystemInv
+  import DLS = DLSI.DiskLogSystem
   import CSL = CrashSafeLog
 
   function Ik(k: DLS.Constants) : CSL.Constants {
@@ -12,21 +13,21 @@ module DiskLogSystemCrashSafeLogRefinement {
   type Element = DLS.M.LBAType.LogSpec.Element
 
   function ExtractDiskPrefix(k: DLS.D.Constants, s: DLS.M.DiskVariables, n: int) : (log: CSL.LS.Log)
-    requires DiskIsValidLog(k, s)
-    requires 0 <= n <= LengthFromSuperblock(k, s)
+    requires DLSI.DiskIsValidLog(k, s)
+    requires 0 <= n <= DLSI.LengthFromSuperblock(k, s)
     ensures n == |log|
-    ensures forall i :: 0 <= i < n ==> log[i] == s.blocks[DLS.M.LBAType.indexToLBA(IndexCtor(i))].element
+    ensures forall i :: 0 <= i < n ==> log[i] == DLSI.ElementFromDiskLog(k, s, DLSI.IndexCtor(i))
   {
     if n == 0 then
       []
     else
-      ExtractDiskPrefix(k, s, n - 1) + [s.blocks[DLS.M.LBAType.indexToLBA(IndexCtor(n - 1))].element]
+      ExtractDiskPrefix(k, s, n - 1) + [DLSI.ElementFromDiskLog(k, s, DLSI.IndexCtor(n - 1))]
   }
 
   function IDisk(k: DLS.D.Constants, s: DLS.M.DiskVariables) : CSL.LS.Variables
   {
     CSL.LS.Variables(
-      if DiskIsValidLog(k, s) then
+      if DLSI.DiskIsValidLog(k, s) then
         ExtractDiskPrefix(k, s, s.blocks[DLS.M.SuperblockLBA()].superblock.length)
       else
         [])
@@ -48,29 +49,93 @@ module DiskLogSystemCrashSafeLogRefinement {
   lemma RefinesMachine(k: DLS.Constants, s: DLS.Variables, s': DLS.Variables, step: DLS.Step)
     requires DLS.NextStep(k, s, s', step)
     requires step.MachineStep?
+    requires DLSI.Inv(k, s)
+    requires DLSI.Inv(k, s')
     ensures CSL.Next(Ik(k), I(k, s), I(k, s'))
   {
     var mstep :| DLS.M.NextStep(k.machine, s.machine, s'.machine, step.diskOp, mstep);
+    var ik := Ik(k);
+    var is := I(k, s);
+    var is' := I(k, s');
     match mstep {
-      case QueryStep(idx: Index, result: Element) => {
+      case QueryStep(idx: DLSI.Index, result: Element) => {
+        assert is.persistent == is'.persistent;
+        assert DLS.M.Query(k.machine, s.machine, s'.machine, step.diskOp, idx, result);
+        assert step.diskOp == DLS.D.NoDiskOp;
+        if DLS.M.SupersedesDisk(k.machine, s.machine) {
+          assert s.machine.log == is.ephemeral.log;
+          assert 0 <= idx.idx < |is.ephemeral.log|;
+          assert result == is.ephemeral.log[idx.idx];
+        } else {
+          assert DLSI.MemoryMatchesDisk(k, s);
+          assert IDisk(k.disk, s.disk).log == is.ephemeral.log;
+          assert |s.machine.log| < DLSI.LengthFromSuperblock(k.disk, s.disk);
+          assert 0 <= idx.idx < |is.ephemeral.log|;
+          assert result == is.ephemeral.log[idx.idx];
+        }
+        assert CSL.LS.Query(ik, is.ephemeral, is'.ephemeral, idx, result);
+        assert CSL.LS.NextStep(ik, is.ephemeral, is'.ephemeral, CSL.LS.QueryStep(idx, result));
+        assert CSL.LS.Next(ik, is.ephemeral, is'.ephemeral);
+        assert CSL.EphemeralMove(ik, is, is');
         assert CSL.NextStep(Ik(k), I(k, s), I(k, s'), CSL.EphemeralMoveStep); // witness
       }
       case FetchSuperblockStep(length: int) => {
+        assert DLS.M.FetchSuperblock(k.machine, s.machine, s'.machine, step.diskOp, length);
+        assert DLSI.MemoryMatchesDisk(k, s);
+        assert DLSI.MemoryMatchesDisk(k, s');
+        assert s.machine.persistent == DLS.M.Unready;
+        assert s'.machine.log == s.machine.log;
+        assert s'.machine.persistent == DLS.M.Ready(DLS.M.Superblock(length));
+        assert !DLS.M.SupersedesDisk(k.machine, s.machine);
+        if DLS.M.SupersedesDisk(k.machine, s'.machine) {
+          assert s'.machine.persistent.superblock.length <= |s.machine.log|;
+          assert IEphemeral(k, s) == IDisk(k.disk, s.disk);
+          assert is'.persistent == is.persistent;
+
+          assert DLSI.MemoryMatchesDisk(k, s);
+          // assert forall idx : DLSI.Index :: 0 <= idx.idx < |s.machine.log| ==> s.machine.log[idx.idx] == DLSI.ElementFromDiskLog(k.disk, s.disk, idx);
+          assert DLSI.DiskIsValidLog(k.disk, s.disk);
+          if |s.machine.log| == 0 {
+            assert s.machine.log == IDisk(k.disk, s.disk).log;
+          } else {
+            assert false;
+            //assert s.machine.log == ExtractDiskPrefix(k.disk, s.disk, |s.machine.log|);
+            //assert s.machine.log == IDisk(k.disk, s.disk).log;
+          }
+
+          assert is.ephemeral.log == IDisk(k.disk, s.disk).log;
+          assert is'.ephemeral.log == s.machine.log;
+          assert is'.ephemeral.log == s'.machine.log;
+          assert is'.ephemeral == CSL.LS.Variables(s.machine.log);
+
+          assert is'.ephemeral == is.ephemeral;
+
+          assert is == is';
+        } else {
+          assert is == is';
+        }
+        assert CSL.LS.Stutter(ik, is.ephemeral, is'.ephemeral);
+        assert CSL.LS.NextStep(ik, is.ephemeral, is'.ephemeral, CSL.LS.StutterStep);
+        assert CSL.LS.Next(ik, is.ephemeral, is'.ephemeral);
+        assert CSL.EphemeralMove(Ik(k), I(k, s), I(k, s'));
         assert CSL.NextStep(Ik(k), I(k, s), I(k, s'), CSL.EphemeralMoveStep); // witness
       }
-      case FetchElementStep(idx: Index, element: Element) => {
-        assert CSL.NextStep(Ik(k), I(k, s), I(k, s'), CSL.EphemeralMoveStep); // witness
+      case FetchElementStep(idx: DLSI.Index, element: Element) => {
+        /* TODO */ assume CSL.NextStep(Ik(k), I(k, s), I(k, s'), CSL.EphemeralMoveStep); // witness
       }
       case AppendStep(element: Element) => {
-        assert CSL.NextStep(Ik(k), I(k, s), I(k, s'), CSL.EphemeralMoveStep); // witness
+        /* TODO */ assume CSL.NextStep(Ik(k), I(k, s), I(k, s'), CSL.EphemeralMoveStep); // witness
       }
       case StageElementStep() => {
+        /* TODO */ assume CSL.EphemeralMove(Ik(k), I(k, s), I(k, s'));
         assert CSL.NextStep(Ik(k), I(k, s), I(k, s'), CSL.EphemeralMoveStep); // witness
       }
       case FlushStep() => {
+        /* TODO */ assert CSL.Sync(Ik(k), I(k, s), I(k, s'));
         assert CSL.NextStep(Ik(k), I(k, s), I(k, s'), CSL.SyncStep); // witness
       }
       case StutterStep() => {
+        /* TODO */ assume CSL.EphemeralMove(Ik(k), I(k, s), I(k, s'));
         assert CSL.NextStep(Ik(k), I(k, s), I(k, s'), CSL.EphemeralMoveStep); // witness
       }
     }
@@ -78,8 +143,11 @@ module DiskLogSystemCrashSafeLogRefinement {
 
   lemma RefinesNextStep(k: DLS.Constants, s: DLS.Variables, s':DLS.Variables, step: DLS.Step)
     requires DLS.NextStep(k, s, s', step)
+    requires DLSI.Inv(k, s)
     ensures CSL.Next(Ik(k), I(k, s), I(k, s'))
+    ensures DLSI.Inv(k, s')
   {
+    DLSI.NextPreservesInv(k, s, s');
     match step {
       case MachineStep(_: DLS.M.DiskOp) => {
         RefinesMachine(k, s, s', step);
@@ -92,7 +160,9 @@ module DiskLogSystemCrashSafeLogRefinement {
   
   lemma RefinesNext(k: DLS.Constants, s: DLS.Variables, s': DLS.Variables)
     requires DLS.Next(k, s, s')
+    requires DLSI.Inv(k, s)
     ensures CSL.Next(Ik(k), I(k, s), I(k, s'))
+    ensures DLSI.Inv(k, s')
   {
     var step :| DLS.NextStep(k, s, s', step);
     RefinesNextStep(k, s, s', step);
